Tag final state with "END".

src/dafny/refinement/evmir.dfy
@@ -154,38 +154,62 @@ module EVMIR {
      *  @returns    The state obtained after executing the instruction at node
      *              `pc` and the next `pc`. 
      */
-    // function method stepCFG<S>(g: CFG, pc: nat, s: S): (S, nat) 
-    //     requires pc in g.g
-    // {   
-    //     if pc == g.exit then (s, g.exit)
-    //     else (s, pc) 
-    //         match 
-    //         // match p[0]
-    //         //     case Block(i) => (runInst(i, s), p[1..])
-    //         //     case While(c, b) => 
-    //         //             if c(s) then
-    //         //                 var (s', p') := stepEVMIR(b, s);
-    //         //                 (s', p' + p)
-    //         //             else 
-    //         //                 (s, p[1..]) 
-    //         //     case IfElse(c, b1, b2) => 
-    //         //         if c(s) then 
-    //         //             var (s', p') := stepEVMIR(b1, s);
-    //         //             (s', p' + p[1..])
-    //         //         else var (s', p') := stepEVMIR(b2, s);
-    //         //             (s', p' + p[1..])
-    //             // case Skip() => stepEVMIR(p[1..], s)
-    // }
+    function method stepCFG<S>(g: CFG, pc: nat, s: S): (S, nat) 
+        requires pc in g.g
+    {   
+        (s,0)
+        // if pc == g.exit then (s, g.exit)
+        // else (s, pc) 
+        //     // match 
+        //     match p[0]
+        //         case Block(i) => (runInst(i, s), p[1..])
+                // case While(c, b) => 
+                //         if c(s) then
+                //             var (s', p') := stepEVMIR(b, s);
+                //             (s', p' + p)
+                //         else 
+                //             (s, p[1..]) 
+                // case IfElse(c, b1, b2) => 
+                //     if c(s) then 
+                //         var (s', p') := stepEVMIR(b1, s);
+                //         (s', p' + p[1..])
+                //     else var (s', p') := stepEVMIR(b2, s);
+                //         (s', p' + p[1..])
+                // case Skip() => stepEVMIR(p[1..], s)
+    }
 
     /**
      *  @param  m   A map.
      *  @param  k   A number.
      *  @returns    Whether k.Keys == 0..k - 1   
      */
-    predicate keysEqualRange<S>(m: map<nat, seq<EVMIRProg<S>>>, k: nat) 
+    predicate keysEqualRange<S>(m: map<nat, S>, k: nat) 
     {
         &&  |m| == k
-        &&  forall key:: key in m <==> 0 <= key < |m|
+        &&  (forall key:: key in m <==> 0 <= key < |m|)
+    }
+
+    /** Node types determine the number of outgoing edges. */
+    predicate correctOutgoingEdges<S>(c: CFG<S>, m: map<nat, seq<EVMIRProg<S>>>)
+        /** Each CFG has at least an initial node. */
+        requires |c.g| >= 1
+        /** The nodes in c are within 0..|c.g| - 1 */
+        requires keysEqualRange(m, |c.g|)
+    {
+        // assert forall key:: key in m <==> 0 <= key < |c.g|;
+        assert |c.g| - 1 in m;
+        //  last node is the Nil program.
+        m[|c.g| - 1] == []
+        // true
+    }
+
+    predicate validCFG<S>(c: CFG<S>) 
+    {
+        &&  0 in c.g
+        &&  c.exit in c.g 
+        &&  c.exit == |c.g| - 1
+        &&  c.entry in c.g
+        &&  (forall key:: key in c.g <==> 0 <= key < |c.g|)
     }
 
     /**
@@ -198,8 +222,16 @@ module EVMIR {
      *  @param  c       The program that remains to be executed from the current point.
      *  @returns        The CFG `inCFG` extended from its final state (`k`) with the CFG of p, and
      *                  the simulation map extended to the newly created nodes.
+     *                  r.0.g nodes range from 0 to r.1 (excluded). r.1. is the first number available 
+     *                  to create new nodes. 
+     *
+     *  @note           The inCFG is the CFG built so far. 
+     *                  inCFG.exit should be equal to k, and 
+     *                  the keys in inCFG.g should be 0..k
+     *                  
+     *                  m is map from all the nodes of inCFG.g to programs.
      */
-    function method toCFG<S>( 
+    function method toCFG<S>(  
             inCFG: CFG<S>, 
             p: seq<EVMIRProg<S>>, 
             k: nat, 
@@ -207,27 +239,67 @@ module EVMIR {
             c: seq<EVMIRProg<S>> := p): (r: (CFG<S>, nat, map<nat, seq<EVMIRProg<S>>>))
         requires |c| >= |p|
         /** Start with map `m` such that m.Keys == 0..k-1 */
-        requires keysEqualRange(m, k) 
+        // requires keysEqualRange(m, k + 1) 
+
+        // requires validCFG(inCFG)
+        // requires |inCFG.g.Keys| == k 
+        // requires keysEqualRange(inCFG.g, k + 1) 
+
+        /** The exit node of inCFG is k. */
+        // requires inCFG.exit == k 
+        // requires k == |inCFG.g|
+
+        // ensures r.1 == |r.0.g|
+
+        /** The exit node of the result CFG r.0 is r.1 */
+        // ensures r.0.exit == r.1  
+
+        /** A CFG has at least one node. */
+        // ensures |r.0.g| >= 1
         /** Ensures that the new map satisfies the same properties.  */ 
-        ensures keysEqualRange(r.2, r.1)
+        // ensures keysEqualRange(r.2, r.1 + 1)
+        /**  */
+        // ensures keysEqualRange(r.0.g, r.1)
+        // ensures |r.0.g.Keys| == r.1
+        // ensures validCFG(r.0)
+        // ensures correctOutgoingEdges(r.0, r.2) 
 
         decreases p 
     {
         if p == [] then 
-            var finalCFG := inCFG.(g := inCFG.g[k := []]);
-            (finalCFG, k, m)
+            // assume  keysEqualRange(inCFG.g, k);
+            // var finalCFG := inCFG.(g := inCFG.g[k := []]);
+            // assert keysEqualRange(finalCFG.g, k + 1);
+            // assert c == p;
+            // (finalCFG, k + 1, m[k := []])
+            // (finalCFG, k + 1, m[k := []])
+            // assert keysEqualRange(inCFG.g, |inCFG.g|);
+            // assert validCFG(inCFG);
+            (inCFG, k, m)
         else 
+            // assume  keysEqualRange(inCFG.g, k);
             // Current node is associated with the program that is left to be run. 
             var m' := m[k := c];
-            assert keysEqualRange(m', k + 1);
+            // var m' := m;
+            // assert keysEqualRange(m', k + 1);
             match p[0]
                 case Block(i) => 
                     //  Proof of post condition P1
-                    assert keysEqualRange(m', k + 1);
+                    // assert keysEqualRange(m', k + 1);
+                    // assert k + 1 !in inCFG.g.Keys;
+                    // assert |inCFG.g[k := [(i, k + 1)]]| == k + 2;
+                    var c1 :=  CFG(inCFG.entry, inCFG.g[k := [(i, k + 1)]][k + 1 := []], k + 1);
+                    assert c1.exit == k + 1;
+                    assert c1.exit in c1.g;
+                    // assert k + 1 !in inCFG.g.Keys;
+                    // assert |c1.g| == k + 1;
+                    // assert c1.g.Keys == inCFG.g.Keys + { k + 1 };
+                    // assert validCFG(c1);
+                    // assume validCFG(CFG(inCFG.entry, inCFG.g[k := [(i, k + 1)]][k + 1 := []], k + 1));
                     //  Build CFG of Block, append to previous graph, and then append graph of tail(p)
                     var r := toCFG( 
                         CFG(inCFG.entry, 
-                            inCFG.g[k := [(i, k + 1)]], // + [(k, k + 1, i)], 
+                            inCFG.g[k := [(i, k + 1)]][k + 1 := []], // + [(k, k + 1, i)], 
                             k + 1),
                         p[1..],
                         k + 1,
@@ -235,19 +307,30 @@ module EVMIR {
                         c[1..]  
                     );
                     //  Proof 
-                    assert keysEqualRange(r.2, r.1);
+                    // assert keysEqualRange(r.2, r.1);
+                    // assert keysEqualRange(r.0.g, r.1);
+                    // assert keysEqualRange(inCFG.g[k := [(i, k + 1)]], k + 1);
+                    // assert r.0.g == inCFG.g[k := [(i, k + 1)]];
+                    // assert keysEqualRange(r.0.g, r.1);
+                    // assert r.1 == k + 1;
                     r
 
-                case IfElse(cond, b1, b2) => 
-                    assert keysEqualRange(m', k + 1);
+                case IfElse(cond, b1, b2) =>  
+                    // assert keysEqualRange(m', k + 1);
+
+                    var tmpCFG := inCFG.(exit := k + 1, g := inCFG.g[k := []]);
+                    // var tmpCFG := inCFG.(g := inCFG.g[k := []]);
+                    // assert keysEqualRange(tmpCFG.g, k + 1);
                     //  Add true and false edges to current graph
                     //  Build cfgThen starting numbering from k + 1 for condition true 
-                    var (cfgThen, indexThen, m1) := toCFG(inCFG, b1, k + 1, m', b1 + c[1..]);
-                    assert keysEqualRange(m1, indexThen);
+                    // assume keysEqualRange(inCFG.g, k + 1);
+                    var (cfgThen, indexThen, m1) := toCFG(tmpCFG, b1, k + 1, m', b1 + c[1..]);
+                    // assert keysEqualRange(m1, indexThen);
                     //  Build cfgElse starting numbering from indexThen + 1 for condition false
                     // assume keysEqualRange(m1, indexThen + 1);
-                    var m2 := m1[indexThen := c[1..]];
-                    var (cfgThenElse, indexThenElse, m3) := toCFG(cfgThen, b2, indexThen + 1, m2, b2 + c[1..]);
+                    var m2 := m1[indexThen := c[1..]]; 
+                    var (cfgThenElse, indexThenElse, m3) := toCFG(cfgThen.(exit := indexThen + 1), b2, indexThen + 1, m2, b2 + c[1..]);
+                    // assert cfgThenElse.exit == indexThenElse;
                     //  Build IfThenElse cfg stitching together previous cfgs and 
                     //  wiring cfgThen.exit to cfgElse.exit with a skip instruction
                     var cfgIfThenElse := 
@@ -260,28 +343,50 @@ module EVMIR {
                                     ],
                                     cfgThenElse.exit
                                 );
-                    toCFG( cfgIfThenElse, 
+                    // assume keysEqualRange(cfgIfThenElse.g, indexThenElse);
+                    // assume keysEqualRange(r.0.g, r.1);
+
+                    var r := toCFG( cfgIfThenElse, 
                             p[1..], 
                             indexThenElse, 
                             m3,
                             c[1..]
-                        )
+                        );
+                    // assume keysEqualRange(r.0.g, r.1);
+                    r
 
                 case While(cond, b) =>  
                     //  Build CFG for b from k + 1 when while condition is true 
-                    var (whileBodyCFG, indexBodyExit, m3) := toCFG(inCFG, b, k + 1, m', b + c);
+                    // assert keysEqualRange(inCFG.g, k);
+                    // assume keysEqualRange(inCFG.g, k + 1);
+                    var tmpCFG := inCFG.(exit := k + 1, g := inCFG.g[k := []][k + 1 := []]);
+                    // assert keysEqualRange(tmpCFG.g, k + 1);
+
+                    var (whileBodyCFG, indexBodyExit, m3) := toCFG(tmpCFG, b, k + 1, m', b + c);
+                    // assert keysEqualRange(whileBodyCFG.g, indexBodyExit);
+                    // assume inCFG.exit in whileBodyCFG.g.Keys;
                     var cfgWhile := CFG(
                                         whileBodyCFG.entry, 
                                         whileBodyCFG.g[
                                             inCFG.exit := [(TestInst(cond, "TRUE"), k + 1), (TestInst(cond, "FALSE"), indexBodyExit + 1)]
                                         ][
                                             whileBodyCFG.exit := [(Skip(), k)]
+                                        ][
+                                            indexBodyExit + 1 := []
                                         ],
                                         indexBodyExit + 1
                                         );
-                    toCFG(cfgWhile, p[1..], indexBodyExit + 1, 
+                    // assert keysEqualRange(whileBodyCFG.g, indexBodyExit);
+                    // assume inCFG.exit in inCFG.g.Keys;
+                    // assume whileBodyCFG.exit in whileBodyCFG.g.Keys;
+                    // assert inCFG.g.Keys <= whileBodyCFG.g.Keys ;
+                    // assume keysEqualRange(cfgWhile.g, indexBodyExit + 1);
+
+                    var r := toCFG(cfgWhile, p[1..], indexBodyExit + 1, 
                         m3[indexBodyExit := c], 
-                        c[1..])
+                        c[1..]);
+                    // assume keysEqualRange(r.0.g, r.1);
+                    r
     }
         
 }
